Access.v
@@ -1,0 +1,211 @@
+(******************************************************************************)
+(*  © Université Lille 1 (2014-2017)                                          *)
+(*                                                                            *)
+(*  This software is a computer program whose purpose is to run a minimal,    *)
+(*  hypervisor relying on proven properties such as memory isolation.         *)
+(*                                                                            *)
+(*  This software is governed by the CeCILL license under French law and      *)
+(*  abiding by the rules of distribution of free software.  You can  use,     *)
+(*  modify and/ or redistribute the software under the terms of the CeCILL    *)
+(*  license as circulated by CEA, CNRS and INRIA at the following URL         *)
+(*  "http://www.cecill.info".                                                 *)
+(*                                                                            *)
+(*  As a counterpart to the access to the source code and  rights to copy,    *)
+(*  modify and redistribute granted by the license, users are provided only   *)
+(*  with a limited warranty  and the software's author,  the holder of the    *)
+(*  economic rights,  and the successive licensors  have only  limited        *)
+(*  liability.                                                                *)
+(*                                                                            *)
+(*  In this respect, the user's attention is drawn to the risks associated    *)
+(*  with loading,  using,  modifying and/or developing or reproducing the     *)
+(*  software by the user in light of its specific status of free software,    *)
+(*  that may mean  that it is complicated to manipulate,  and  that  also     *)
+(*  therefore means  that it is reserved for developers  and  experienced     *)
+(*  professionals having in-depth computer knowledge. Users are therefore     *)
+(*  encouraged to load and test the software's suitability as regards their   *)
+(*  requirements in conditions enabling the security of their systems and/or  *)
+(*  data to be ensured and,  more generally, to use and operate it in the     *)
+(*  same conditions as regards security.                                      *)
+(*                                                                            *)
+(*  The fact that you are presently reading this means that you have had      *)
+(*  knowledge of the CeCILL license and that you accept its terms.            *)
+(******************************************************************************)
+
+Require Import List Arith NPeano Coq.Logic.JMeq Coq.Logic.Classical_Prop.
+Import List.ListNotations .
+Require Import Lib StateMonad HMonad MMU Alloc_invariants
+ Properties LibOs PageTableManager MemoryManager MMU_invariant.
+Require Import Coq.Structures.OrderedTypeEx.
+
+Set Printing Projections.
+(** * Read a value at a given physical address *)
+Definition read_phy_addr (phy_addr : nat) := 
+  perform s := get in 
+               if lt_dec phy_addr  (length s.(data))  
+               then ret (inl (List.nth phy_addr s.(data) 0))
+               else ret (inr tt).
+
+Lemma read_phy_addr_wp (phys_addr : nat) (P : nat+unit -> state -> Prop) :
+  {{ fun s => phys_addr < length s.(data) /\ 
+ P (inl (List.nth phys_addr s.(data) 0)) s \/ phys_addr >= length s.(data)  /\ P (inr tt) s}} 
+read_phy_addr phys_addr {{ P }}.
+Proof.
+unfold read_phy_addr.
+eapply bind_wp.
+intros s. 
+
+instantiate (1 := fun s' s =>s = s' /\ (phys_addr < length s.(data) /\ 
+ P (inl (List.nth phys_addr s.(data) 0)) s \/ phys_addr >= length s.(data)  /\ P (inr tt) s)).
+   simpl. 
+case_eq (lt_dec phys_addr (length (data s))).
+ + intros.
+   eapply weaken.
+   eapply ret_wp.
+   intros.
+   simpl.
+   destruct H0. 
+   subst. 
+   intuition.
+   contradict H1.
+   intuition.
+ + intros. 
+   eapply weaken.
+   apply ret_wp.
+   intros.
+   destruct H0.
+   subst. 
+   intuition.
+   contradict H1.
+   intuition.
+ + eapply weaken.
+   eapply get_wp.
+   intros.
+   simpl.
+   destruct H. 
+   intuition.
+   intuition.
+Qed.
+
+
+
+
+Definition read ( Vaddr : nat):  M (nat+unit):= 
+
+perform Paddr := translate Vaddr in 
+match Paddr with 
+|inl paddr => read_phy_addr paddr
+|inr faultpage => ret (inr tt)
+|inr noaccess => ret (inr tt)
+end.
+ 
+
+
+
+
+(** * assignment of the register with a value *)
+
+Definition assign (v : nat) : M unit :=
+  modify (fun s => {|
+    process_list := s.(process_list);
+    current_process := s.(current_process);
+    cr3 := s.(cr3);
+    intr_table := s.(intr_table);
+    interruptions := s.(interruptions);
+    kernel_mode := s.(kernel_mode);
+    pc := s.(pc);
+    code := s.(code);
+    stack := s.(stack);
+    register := v;
+    first_free_page := s.(first_free_page);
+    data := s.(data)    
+  |}
+).
+
+Lemma assign_wp (v : nat) (P : unit -> state -> Prop) :
+  {{ fun s => P tt {|
+      process_list := s.(process_list);
+      current_process := s.(current_process);
+      cr3 := s.(cr3);
+      intr_table := s.(intr_table);
+      interruptions := s.(interruptions);
+      kernel_mode := s.(kernel_mode);
+      pc := s.(pc);
+      code := s.(code);
+      stack := s.(stack);
+      register := v;
+      first_free_page := s.(first_free_page);
+      data := s.(data)    
+  |}
+}} assign v {{ P }}.
+Proof.
+apply modify_wp.
+Qed.
+
+
+
+
+
+(** * put in the regester the value at the physical address .
+  *)
+
+Definition load (Vaddr : nat) : M unit :=
+perform value := read Vaddr in 
+match value with 
+|inl v =>  assign v
+|inr _ => assign 0 
+end.
+
+Definition write_aux (val Paddr: nat) := 
+let page := getBase Paddr offset_nb_bits in 
+let index := getOffset Paddr offset_nb_bits in  
+ modify (fun s =>  {|
+    process_list := s.(process_list);
+    current_process := s.(current_process);
+    cr3 := s.(cr3);
+    intr_table := s.(intr_table);
+    interruptions := s.(interruptions);
+    kernel_mode := s.(kernel_mode);
+    pc := s.(pc);
+    code := s.(code);
+    stack := s.(stack);
+    register := s.(register);
+    first_free_page := s.(first_free_page);
+    data := firstn (page * page_size) s.(data) ++
+             update_sublist index val
+               (sublist (page * page_size) page_size s.(data)) ++
+             skipn (page * page_size + nb_pte) s.(data)   
+|}).
+Lemma write_aux_wp (val Paddr: nat) (P : unit-> state-> Prop) :
+let page := getBase Paddr offset_nb_bits in 
+let index := getOffset Paddr offset_nb_bits in  
+{{fun s => P tt {|
+    process_list := s.(process_list);
+    current_process := s.(current_process);
+    cr3 := s.(cr3);
+    intr_table := s.(intr_table);
+    interruptions := s.(interruptions);
+    kernel_mode := s.(kernel_mode);
+    pc := s.(pc);
+    code := s.(code);
+    stack := s.(stack);
+    register := s.(register);
+    first_free_page := s.(first_free_page);
+    data := firstn (page * page_size) s.(data) ++
+             update_sublist index val
+               (sublist (page * page_size) page_size s.(data)) ++
+             skipn (page * page_size + nb_pte) s.(data) |}
+}}
+write_aux val Paddr {{ P }}.
+Proof.
+simpl.
+apply modify_wp.
+Qed.
+
+
+Definition write (val Vaddr : nat) := 
+perform Paddr := translate Vaddr in 
+match Paddr with 
+|inl paddr => write_aux val paddr
+|inr _ => ret tt
+end.
+
